@prefix : <http://data.europa.eu2sa/cssv#> .
@prefix cc: <http://creativecommons.org/ns#> .
@prefix dc: <http://www.omg.org/spec/UML/20131001/UMLDC> .
@prefix dct: <http://purl.org/dc/terms/> .
@prefix org: <http://www.w3.org/ns/org#> .
@prefix owl: <http://www.w3.org/2002/07/owl#> .
@prefix pav: <http://purl.org/pav/> .
@prefix rdf: <http://www.w3.org/1999/02/22-rdf-syntax-ns#> .
@prefix sch: <https://schema.org/> .
@prefix xml: <http://www.w3.org/XML/1998/namespace> .
@prefix xsd: <http://www.w3.org/2001/XMLSchema#> .
@prefix cssv: <http://data.europa.eu2sa/cssv#> .
@prefix dcat: <http://www.w3.org/ns/dcat#> .
@prefix foaf: <http://xmlns.com/foaf/0.1/> .
@prefix prof: <https://www.w3.org/TR/dx-prof/#> .
@prefix rdfs: <http://www.w3.org/2000/01/rdf-schema#> .
@prefix skos: <http://www.w3.org/2004/02/skos/core#> .
@prefix vann: <http://purl.org/vocab/vann/> .
@base <http://data.europa.eu2sa/cssv#> .

<http://data.europa.eu2sa/cssv#> rdf:type owl:Ontology ;
                                  owl:versionIRI cssv: ;
                                  owl:imports dct: ,
                                    rdfs: ,
                                    skos: ,
                                    dcat: ,
                                    foaf: ;
                                  cc:attributionName "European Commission" ;
                                  dct:description "This module provides the definitions for the Core Standards and Specifications Vocabulary."@en ;
                                  dct:date "2024-11-29" ;
                                  dct:license <http://creativecommons.org/licenses/by-sa/4.0/> ;
                                  dct:mediator [ foaf:name "Common Assessment Method for Standards and Specifications (CAMSS)" ;
                                                 foaf:homepage "https://interoperable-europe.ec.europa.eu/collection/common-assessment-method-standards-and-specifications-camss"
                                               ] ;
                                  dct:title "Core Standards and Specifications Vocabulary"@en ;
                                  vann:preferredNamespacePrefix "cssv" ;
                                  vann:preferredNamespaceUri "http://data.europa.eu2sa/cssv#" ;
                                  rdfs:label "Core Standards and Specifications Vocabulary" ;
                                  rdfs:seeAlso <https://github.com/isa-camss/CSSV> ,
                                               <https://joinup.ec.europa.eu/collection/common-assessment-method-standards-and-specifications-camss/solution/core-standards-and-specifications-vocabulary-cssv> ;
                                  owl:versionInfo "1.4.0" ;
                                  skos:note "This file has been generated with Protégé." ;
                                  foaf:maker [ rdf:type foaf:Person ;
                                               foaf:firstName "Common Assessment Method for Standards and Specifications (CAMSS)"
                                              ] .

#################################################################
#    Datatypes
#################################################################

###  http://www.w3.org/2000/01/rdf-schema#Literal
rdfs:Literal owl:equivalentClass rdf:langString ,
                                 xsd:date ,
                                 xsd:dateTime ,
                                 xsd:decimal ,
                                 xsd:int ,
                                 xsd:string .


###  http://www.w3.org/2001/XMLSchema#date
xsd:date rdf:type rdfs:Datatype .


###  http://www.w3.org/2004/02/skos/core#Concept
skos:Concept rdf:type rdfs:Datatype .

rdfs:Resource rdf:type rdfs:Literal .


#################################################################
#    Object Properties
#################################################################

###  http://purl.org/dc/terms/creator
dct:creator rdf:type owl:ObjectProperty ;
            rdfs:domain dcat:Resource ;
            rdfs:range org:Organization .


###  http://purl.org/pav/http://www.w3.org/ns/dcat#previousVersion
dcat:previousVersion rdf:type owl:ObjectProperty ;
            rdfs:domain cssv:Specification ;
            rdfs:range cssv:Specification ;
            rdfs:comment "The previous version of a resource in a lineage."@en ;
            rdfs:isDefinedBy <https://www.w3.org/ns/dcat#> ;
            rdfs:label "Previous version"@en ;
            skos:definition "The previous version of a resource in a lineage."@en ;
            skos:prefLabel "Previous version"@en .


###  http://www.w3.org/ns/dcat#distribution
dcat:distribution rdf:type owl:ObjectProperty ;
                  rdfs:domain dcat:Dataset ;
                  rdfs:range dcat:Distribution .


###  http://www.w3.org/ns/dcat#theme
dcat:theme rdf:type owl:ObjectProperty ;
           rdfs:domain dcat:Resource .


###  http://data.europa.eu2sa/cssv#combinedIn
cssv:combinedIn rdf:type owl:ObjectProperty ;
                owl:inverseOf cssv:combines ;
                rdfs:domain cssv:Specification ;
                rdfs:range cssv:Family ;
                rdfs:comment "A set of Specifications that are complementary and interrelated, forming a Family of Specifications."@en ;
                rdfs:isDefinedBy <http://data.europa.eu/w21/e1f84ab1-bad6-4e95-b37a-e54ba7dfc551> ;
                skos:definition "A set of Specifications that are complementary and interrelated, forming a Family of Specifications."@en ;
                skos:prefLabel "Combined in"@en .


###  http://data.europa.eu2sa/cssv#combines
cssv:combines rdf:type owl:ObjectProperty ;
              rdfs:domain cssv:Family ;
              rdfs:range cssv:Specification ;
              rdfs:comment "Whether a Family is a union of more than one Specifications."@en ;
              rdfs:isDefinedBy <http://data.europa.eu/w21/e1f84ab1-bad6-4e95-b37a-e54ba7dfc551> ;
              skos:definition "Whether a Family is a union of more than one Specifications."@en ;
              skos:prefLabel "Combines"@en .


###  http://data.europa.eu2sa/cssv#configuredIn
cssv:configuredIn rdf:type owl:ObjectProperty ;
                  owl:inverseOf cssv:configures ;
                  rdfs:domain cssv:Specification ;
                  rdfs:range cssv:ApplicationProfile ;
                  rdfs:comment "A set of Specifications potentially for a given use case or policy domain that are aggregated in an ApplicationProfile."@en ;
                  rdfs:isDefinedBy <http://data.europa.eu/w21/e1f84ab1-bad6-4e95-b37a-e54ba7dfc551> ;
                  skos:definition "A set of Specifications potentially for a given use case or policy domain that are aggregated in an ApplicationProfile."@en ;
                  skos:prefLabel "Configured in"@en .


###  http://data.europa.eu2sa/cssv#configures
cssv:configures rdf:type owl:ObjectProperty ;
                rdfs:domain cssv:ApplicationProfile ;
                rdfs:range cssv:Specification ;
                rdfs:comment "Whether an Application Profile design or adapts a Specification for a specific purpose."@en ;
                rdfs:isDefinedBy <http://data.europa.eu/w21/e1f84ab1-bad6-4e95-b37a-e54ba7dfc551> ;
                skos:definition "Whether an Application Profile design or adapts a Specification for a specific purpose."@en ;
                skos:prefLabel "Configures"@en .


###  http://data.europa.eu2sa/cssv#isAspectOf
cssv:isAspectOf rdf:type owl:ObjectProperty ;
                rdfs:domain cssv:ApplicationProfile ;
                rdfs:range prof:Profile ;
                rdfs:comment "ApplicationProfile is a part of a Profile."@en ;
                rdfs:isDefinedBy <http://data.europa.eu/w21/e1f84ab1-bad6-4e95-b37a-e54ba7dfc551> ;
                skos:definition "ApplicationProfile is a part of a Profile."@en ;
                skos:prefLabel "Is aspect of"@en .

###  http://data.europa.eu2sa/cssv#isMaintainedBy
cssv:isMaintainedBy rdf:type owl:ObjectProperty ;
                    rdfs:domain cssv:Specification ;
                    rdfs:range foaf:Agent ;
                    rdfs:comment "The Person, Organisation reponsible to update and maintain the specification."@en ;
                    rdfs:isDefinedBy <http://data.europa.eu/w21/e1f84ab1-bad6-4e95-b37a-e54ba7dfc551> ;
                    skos:definition "The Person, Organisation reponsible to update and maintain the specification."@en ;
                    skos:prefLabel "Is maintained by"@en .


###  http://data.europa.eu2sa/cssv#isRecommendedBy
cssv:isRecommendedBy rdf:type owl:ObjectProperty ;
                     rdfs:domain cssv:Specification ;
                     rdfs:range foaf:Agent ;
                     rdfs:comment "A link to any other person or organisation that recommends the specification." ;
                     rdfs:isDefinedBy <http://data.europa.eu/w21/e1f84ab1-bad6-4e95-b37a-e54ba7dfc551> ;
                     rdfs:label "Is recommended by" ;
                     skos:definition "A link to any other person or organisation that recommends the specification." ;
                     skos:prefLabel "Is recommended by" .


###  https://schema.org/contactPoint
sch:contactPoint rdf:type owl:ObjectProperty ;
                 rdfs:domain sch:ContactPoint ;
                 rdfs:range org:Organization .


#################################################################
#    Data properties
#################################################################

###  http://purl.org/dc/terms/accessRights
dct:accessRights rdf:type owl:DatatypeProperty ;
                 rdfs:domain dcat:Resource ;
                 rdfs:range rdfs:Literal .


###  http://purl.org/dc/terms/description
dct:description rdf:type owl:DatatypeProperty ;
                rdfs:domain cssv:Specification ;
                rdfs:range rdfs:Literal .


###  http://purl.org/dc/terms/identifier
dct:identifier rdf:type owl:DatatypeProperty ;
               rdfs:domain cssv:Specification ;
               rdfs:range rdfs:Literal .


###  http://purl.org/dc/terms/license
dct:license rdf:type owl:DatatypeProperty ;
            rdfs:domain dcat:Resource ;
            rdfs:range rdfs:Literal .


###  http://purl.org/dc/terms/rights
dct:rights rdf:type owl:DatatypeProperty ;
           rdfs:domain dcat:Resource ;
           rdfs:range rdfs:Literal .


###  http://purl.org/dc/terms/title
dct:title rdf:type owl:DatatypeProperty ;
          rdfs:domain cssv:Specification ;
          rdfs:range rdfs:Literal .


###  http://purl.org/dc/terms/type
dct:type rdf:type owl:DatatypeProperty ;
         rdfs:domain cssv:Specification ;
         rdfs:range skos:Concept .


###  http://purl.org/pav/http://www.w3.org/ns/dcat#version
dcat:version rdf:type owl:DatatypeProperty ;
        rdfs:domain cssv:Specification ;
        rdfs:range rdfs:Literal ;
        rdfs:comment "The version indicator (name or identifier) of a resource."@en ;
        rdfs:isDefinedBy dcat: ;
        rdfs:label "Version"@en ;
        skos:definition "The version indicator (name or identifier) of a resource."@en ;
        skos:prefLabel "Version"@en .


###  http://www.w3.org/ns/dcat#accessURL
dcat:accessURL rdf:type owl:DatatypeProperty ;
               rdfs:domain dcat:Distribution ;
               rdfs:range rdfs:Literal .


###  http://www.w3.org/ns/dcat#downloadURL
dcat:downloadURL rdf:type owl:DatatypeProperty ;
                 rdfs:domain dcat:Distribution ;
                 rdfs:range rdfs:Literal .


###  http://data.europa.eu2sa/cssv#acronym
cssv:acronym rdf:type owl:DatatypeProperty ;
             rdfs:domain cssv:Specification ;
             rdfs:range rdfs:Literal ;
             rdfs:comment "Abbreviation of the specification."@en ;
             rdfs:isDefinedBy cssv: ;
             skos:altLabel "Has acronym"@en ;
             skos:definition "Abbreviation of the specification."@en ;
             skos:prefLabel "Acronym"@en .


###  http://data.europa.eu2sa/cssv#alternative
cssv:alternative rdf:type owl:DatatypeProperty ;
                 rdfs:domain cssv:Specification ;
                 rdfs:range rdfs:Literal ;
                 rdfs:comment "The alternative name of the specification."@en ;
                 rdfs:isDefinedBy cssv: ;
                 skos:definition "The alternative name of the specification."@en ;
                 skos:prefLabel "Alternative"@en .


#################################################################
#    Classes
#################################################################

###  http://purl.org/dc/terms/Standard
dct:Standard rdf:type owl:Class .


###  http://www.w3.org/ns/dcat#Dataset
dcat:Dataset rdf:type owl:Class ;
             rdfs:subClassOf dcat:Resource .


###  http://www.w3.org/ns/dcat#Distribution
dcat:Distribution rdf:type owl:Class .


###  http://www.w3.org/ns/dcat#Resource
dcat:Resource rdf:type owl:Class .


###  http://www.w3.org/ns/org#Organization
org:Organization rdf:type owl:Class ;
                 rdfs:subClassOf foaf:Agent .


###  http://xmlns.com/foaf/0.1/Agent
foaf:Agent rdf:type owl:Class .


###  http://data.europa.eu2sa/cssv#ApplicationProfile
cssv:ApplicationProfile rdf:type owl:Class ;
                        rdfs:subClassOf cssv:Specification ;
                        owl:disjointWith cssv:Family ,
                                         cssv:Standard ;
                        rdfs:comment "An application profile “customises one or more existing specifications potentially for a given use case or a policy domain adding an end to end narrative describing and ensuring the interoperability of its underlying specification(s)”."@en ;
                        rdfs:isDefinedBy <http://data.europa.eu/w21/e1f84ab1-bad6-4e95-b37a-e54ba7dfc551> ;
                        skos:definition "An application profile “customises one or more existing specifications potentially for a given use case or a policy domain adding an end to end narrative describing and ensuring the interoperability of its underlying specification(s)”."@en ;
                        skos:prefLabel "Application Profile"@en .


###  http://data.europa.eu2sa/cssv#Family
cssv:Family rdf:type owl:Class ;
            rdfs:subClassOf cssv:Specification ;
            owl:disjointWith cssv:Standard ;
            rdfs:comment "A collection of interrelated and/or complementary specifications, standards or application profiles and the explanation of how they are combined, used or both."@en ;
            rdfs:isDefinedBy <http://data.europa.eu/w21/e1f84ab1-bad6-4e95-b37a-e54ba7dfc551> ;
            skos:definition "A collection of interrelated and/or complementary specifications, standards or application profiles and the explanation of how they are combined, used or both."@en ;
            skos:prefLabel "Family"@en .


###  http://data.europa.eu2sa/cssv#Specification
cssv:Specification rdf:type owl:Class ;
                   rdfs:subClassOf dcat:Dataset ;
                   rdfs:comment "Document with normative guidelines or characteristics that can be used consistently to ensure that materials, products, processes and services conform to one or a set of requirements (ISO). Specifications are the cornerstone of interoperability, as they set the grounds for the design and development of interoperable and reusable solutions based in common services at the lowest level."@en ;
                   rdfs:isDefinedBy <http://data.europa.eu/w21/e1f84ab1-bad6-4e95-b37a-e54ba7dfc551> ;
                   skos:definition "Precise requirements that are needed for the implementation of a solution. A specification is not necessarily a standard."@en ;
                   skos:prefLabel "Specification"@en .


###  http://data.europa.eu2sa/cssv#Standard
cssv:Standard rdf:type owl:Class ;
              rdfs:subClassOf dct:Standard ,
                              cssv:Specification ;
              rdfs:comment "Specification that has reached a certain maturity and widespread adoption and potentially endorsed."@en ;
              rdfs:isDefinedBy <http://data.europa.eu/w21/e1f84ab1-bad6-4e95-b37a-e54ba7dfc551> ;
              skos:definition "Specification that has reached a certain maturity and widespread adoption and potentially endorsed."@en ;
              skos:prefLabel "Standard"@en .


###  https://schema.org/ContactPoint
sch:ContactPoint rdf:type owl:Class .


###  https://www.w3.org/TR/dx-prof/#Profile
prof:Profile rdf:type owl:Class ;
             rdfs:subClassOf dct:Standard .