@prefix : <https://data.europa.eu2sa/cssv#> .
@prefix cc: <http://creativecommons.org/ns#> .
@prefix dc: <http://www.omg.org/spec/UML/20131001/UMLDC> .
@prefix dct: <http://purl.org/dc/terms/> .
@prefix org: <http://www.w3.org/ns/org#> .
@prefix owl: <http://www.w3.org/2002/07/owl#> .
@prefix pav: <http://purl.org/pav/> .
@prefix rdf: <http://www.w3.org/1999/02/22-rdf-syntax-ns#> .
@prefix sch: <https://schema.org/> .
@prefix xml: <http://www.w3.org/XML/1998/namespace> .
@prefix xsd: <http://www.w3.org/2001/XMLSchema#> .
@prefix cssv: <https://data.europa.eu2sa/cssv#> .
@prefix dcat: <http://www.w3.org/ns/dcat#> .
@prefix foaf: <http://xmlns.com/foaf/0.1/> .
@prefix prof: <https://www.w3.org/TR/dx-prof/#> .
@prefix rdfs: <http://www.w3.org/2000/01/rdf-schema#> .
@prefix skos: <http://www.w3.org/2004/02/skos/core#> .
@prefix vann: <http://purl.org/vocab/vann/> .
@base <https://data.europa.eu2sa/cssv#> .

<https://data.europa.eu2sa/cssv> rdf:type owl:Ontology ;
                                  owl:versionIRI cssv:CSSV.ttl ;
                                  cc:attributionName "European Commission - ISA2, CAMSS Team" ;
                                  dct:date "2022-03-31"^^xsd:date ;
                                  vann:preferredNamespacePrefix "cssv" ;
                                  vann:preferredNamespaceUri "https://data.europa.eu2sa/cssv#" ;
                                  rdfs:label "Core Standards and Specifications Vocabulary"@en ;
                                  rdfs:seeAlso <https://github.com/isa-camss/CSSV> ,
                                               <https://joinup.ec.europa.eu/collection/common-assessment-method-standards-and-specifications-camss/solution/core-standards-and-specifications-vocabulary-cssv> ,
                                               <https://joinup.ec.europa.eu/collection/semantic-interoperability-community-semic/solution/e-government-core-vocabularies/core-standards-and-specifications-vocabulary> ;
                                  owl:versionInfo "1.3.0" .

#################################################################
#    Annotation properties
#################################################################

###  http://creativecommons.org/ns#attributionName
cc:attributionName rdf:type owl:AnnotationProperty .


###  http://purl.org/dc/terms/date
dct:date rdf:type owl:AnnotationProperty .


###  http://purl.org/vocab/vann/preferredNamespacePrefix
vann:preferredNamespacePrefix rdf:type owl:AnnotationProperty .


###  http://purl.org/vocab/vann/preferredNamespaceUri
vann:preferredNamespaceUri rdf:type owl:AnnotationProperty .


###  http://www.w3.org/2004/02/skos/core#altLabel
skos:altLabel rdf:type owl:AnnotationProperty .


###  http://www.w3.org/2004/02/skos/core#definition
skos:definition rdf:type owl:AnnotationProperty .


###  http://www.w3.org/2004/02/skos/core#prefLabel
skos:prefLabel rdf:type owl:AnnotationProperty .


#################################################################
#    Datatypes
#################################################################

###  http://www.w3.org/2001/XMLSchema#date
xsd:date rdf:type rdfs:Datatype .


###  http://www.w3.org/2004/02/skos/core#Concept
skos:Concept rdf:type rdfs:Datatype .


#################################################################
#    Object Properties
#################################################################

###  http://purl.org/dc/terms/creator
dct:creator rdf:type owl:ObjectProperty ;
            rdfs:domain dcat:Resource ;
            rdfs:range org:Organization .


###  http://purl.org/pav/previousVersion
pav:previousVersion rdf:type owl:ObjectProperty ;
                    rdfs:domain cssv:Specification ;
                    rdfs:range cssv:Specification .


###  http://www.w3.org/ns/dcat#distribution
dcat:distribution rdf:type owl:ObjectProperty ;
                  rdfs:domain dcat:Dataset ;
                  rdfs:range dcat:Distribution .


###  http://www.w3.org/ns/dcat#theme
dcat:theme rdf:type owl:ObjectProperty ;
           rdfs:domain dcat:Resource .


###  https://data.europa.eu2sa/cssv#combinedIn
cssv:combinedIn rdf:type owl:ObjectProperty ;
                owl:inverseOf cssv:combines ;
                rdfs:domain cssv:Specification ;
                rdfs:range cssv:Family ;
                rdfs:comment "A set of Specifications that are complementary and interrelated, forming a Family of Specifications."@en ;
                rdfs:isDefinedBy <https://data.europa.eu2sa/cssv> ;
                rdfs:label "Combined in"@en ;
                skos:definition "A set of Specifications that are complementary and interrelated, forming a Family of Specifications."@en ;
                skos:prefLabel "Combined in"@en .


###  https://data.europa.eu2sa/cssv#combines
cssv:combines rdf:type owl:ObjectProperty ;
              rdfs:domain cssv:Family ;
              rdfs:range cssv:Specification ;
              rdfs:comment "Whether a Family is a union of more than one Specifications."@en ;
              rdfs:isDefinedBy <https://data.europa.eu2sa/cssv> ;
              rdfs:label "Combines"@en ;
              skos:definition "Whether a Family is a union of more than one Specifications."@en ;
              skos:prefLabel "Combines"@en .


###  https://data.europa.eu2sa/cssv#configuredIn
cssv:configuredIn rdf:type owl:ObjectProperty ;
                  owl:inverseOf cssv:configures ;
                  rdfs:domain cssv:Specification ;
                  rdfs:range cssv:ApplicationProfile ;
                  rdfs:comment "A set of Specifications potentially for a given use case or policy domain that are aggregated in an ApplicationProfile."@en ;
                  rdfs:isDefinedBy <https://data.europa.eu2sa/cssv> ;
                  rdfs:label "Configured in"@en ;
                  skos:definition "A set of Specifications potentially for a given use case or policy domain that are aggregated in an ApplicationProfile."@en ;
                  skos:prefLabel "Configured in"@en .


###  https://data.europa.eu2sa/cssv#configures
cssv:configures rdf:type owl:ObjectProperty ;
                rdfs:domain cssv:ApplicationProfile ;
                rdfs:range cssv:Specification ;
                rdfs:comment "Whether an Application Profile design or adapts a Specification for a specific purpose."@en ;
                rdfs:isDefinedBy <https://data.europa.eu2sa/cssv> ;
                rdfs:label "Configures"@en ;
                skos:definition "Whether an Application Profile design or adapts a Specification for a specific purpose."@en ;
                skos:prefLabel "Configures"@en .


###  https://data.europa.eu2sa/cssv#isAspectOf
cssv:isAspectOf rdf:type owl:ObjectProperty ;
                rdfs:domain cssv:ApplicationProfile ;
                rdfs:range prof:Profile ;
                rdfs:comment "ApplicationProfile is a part of a Profile."@en ;
                rdfs:isDefinedBy <https://data.europa.eu2sa/cssv> ;
                rdfs:label "Is aspect of"@en ;
                skos:definition "ApplicationProfile is a part of a Profile."@en ;
                skos:prefLabel "Is aspect of"@en .


###  https://data.europa.eu2sa/cssv#isContactPointOf
cssv:isContactPointOf rdf:type owl:ObjectProperty ;
                      rdfs:domain sch:ContactPoint ;
                      rdfs:range foaf:Agent ;
                      rdfs:comment "The ContactPoint is an instance of a subclass of foaf:Agent (e.g. an org:Organization)."@en ;
                      rdfs:isDefinedBy <https://data.europa.eu2sa/cssv> ;
                      rdfs:label "Is contact point of"@en ;
                      owl:deprecated "Deprecated. Replaced by schema:contactPoint"@en ;
                      skos:definition "The ContactPoint is an instance of a subclass of foaf:Agent (e.g. an org:Organization)."@en ;
                      skos:prefLabel "Is contact point of"@en .


###  https://data.europa.eu2sa/cssv#isMaintainedBy
cssv:isMaintainedBy rdf:type owl:ObjectProperty ;
                    rdfs:domain cssv:Specification ;
                    rdfs:range foaf:Agent ;
                    rdfs:comment "The Person, Organisation reponsible to update and maintain the specification."@en ;
                    rdfs:isDefinedBy <https://data.europa.eu2sa/cssv> ;
                    rdfs:label "Is maintained by"@en ;
                    skos:definition "The Person, Organisation reponsible to update and maintain the specification."@en ;
                    skos:prefLabel "Is maintained by"@en .


###  https://schema.org/contactPoint
sch:contactPoint rdf:type owl:ObjectProperty ;
                 rdfs:domain sch:ContactPoint ;
                 rdfs:range org:Organization .


#################################################################
#    Data properties
#################################################################

###  http://purl.org/dc/terms/accessRights
dct:accessRights rdf:type owl:DatatypeProperty ;
                 rdfs:domain dcat:Resource ;
                 rdfs:range xsd:anyURI .


###  http://purl.org/dc/terms/description
dct:description rdf:type owl:DatatypeProperty ;
                rdfs:domain cssv:Specification ;
                rdfs:range xsd:string .


###  http://purl.org/dc/terms/identifier
dct:identifier rdf:type owl:DatatypeProperty ;
               rdfs:domain cssv:Specification ;
               rdfs:range xsd:anyURI .


###  http://purl.org/dc/terms/license
dct:license rdf:type owl:DatatypeProperty ;
            rdfs:domain dcat:Resource ;
            rdfs:range xsd:anyURI .


###  http://purl.org/dc/terms/rights
dct:rights rdf:type owl:DatatypeProperty ;
           rdfs:domain dcat:Resource ;
           rdfs:range xsd:anyURI .


###  http://purl.org/dc/terms/title
dct:title rdf:type owl:DatatypeProperty ;
          rdfs:domain cssv:Specification ;
          rdfs:range xsd:string .


###  http://purl.org/dc/terms/type
dct:type rdf:type owl:DatatypeProperty ;
         rdfs:domain cssv:Specification ;
         rdfs:range skos:Concept .


###  http://purl.org/pav/version
pav:version rdf:type owl:DatatypeProperty ;
            rdfs:domain cssv:Specification ;
            rdfs:range xsd:string ;
            rdfs:comment "The version number of a resource. This is a freetext string, typical values are \"1.5\" or \"21\". The URI identifying the previous version can be provided using prov:previousVersion."@en ;
            rdfs:isDefinedBy pav: ;
            rdfs:label "Previous version"@en ;
            skos:definition "The version number of a resource. This is a freetext string, typical values are \"1.5\" or \"21\". The URI identifying the previous version can be provided using prov:previousVersion."@en ;
            skos:prefLabel "Previous version"@en .


###  http://www.w3.org/ns/dcat#accessURL
dcat:accessURL rdf:type owl:DatatypeProperty ;
               rdfs:domain dcat:Distribution ;
               rdfs:range xsd:anyURI .


###  http://www.w3.org/ns/dcat#downloadURL
dcat:downloadURL rdf:type owl:DatatypeProperty ;
                 rdfs:domain dcat:Distribution ;
                 rdfs:range xsd:anyURI .


###  https://data.europa.eu2sa/cssv#acronym
cssv:acronym rdf:type owl:DatatypeProperty ;
             rdfs:domain cssv:Specification ;
             rdfs:range xsd:string ;
             rdfs:comment "Abbreviation of the specification."@en ;
             rdfs:isDefinedBy cssv: ;
             skos:altLabel "Has acronym"@en ;
             skos:definition "Abbreviation of the specification."@en ;
             skos:prefLabel "Acronym"@en .


###  https://data.europa.eu2sa/cssv#alternative
cssv:alternative rdf:type owl:DatatypeProperty ;
                 rdfs:domain cssv:Specification ;
                 rdfs:range xsd:string ;
                 rdfs:comment "The alternative name of the specification."@en ;
                 rdfs:isDefinedBy cssv: ;
                 rdfs:label "Alternative"@en ;
                 skos:definition "The alternative name of the specification."@en ;
                 skos:prefLabel "Alternative"@en .


#################################################################
#    Classes
#################################################################

###  http://purl.org/dc/terms/Standard
dct:Standard rdf:type owl:Class .


###  http://www.w3.org/ns/dcat#Dataset
dcat:Dataset rdf:type owl:Class ;
             rdfs:subClassOf dcat:Resource .


###  http://www.w3.org/ns/dcat#Distribution
dcat:Distribution rdf:type owl:Class .


###  http://www.w3.org/ns/dcat#Resource
dcat:Resource rdf:type owl:Class .


###  http://www.w3.org/ns/org#Organization
org:Organization rdf:type owl:Class ;
                 rdfs:subClassOf foaf:Agent .


###  http://xmlns.com/foaf/0.1/Agent
foaf:Agent rdf:type owl:Class .


###  https://data.europa.eu2sa/cssv#ApplicationProfile
cssv:ApplicationProfile rdf:type owl:Class ;
                        rdfs:subClassOf cssv:Specification ;
                        owl:disjointWith cssv:Family ,
                                         cssv:Standard ;
                        rdfs:comment "An application profile “customises one or more existing specifications potentially for a given use case or a policy domain adding an end to end narrative describing and ensuring the interoperability of its underlying specification(s)”."@en ;
                        rdfs:isDefinedBy <https://data.europa.eu2sa/cssv> ;
                        rdfs:label "Application Profile"@en ;
                        skos:definition "An application profile “customises one or more existing specifications potentially for a given use case or a policy domain adding an end to end narrative describing and ensuring the interoperability of its underlying specification(s)”."@en ;
                        skos:prefLabel "Application Profile"@en .


###  https://data.europa.eu2sa/cssv#Family
cssv:Family rdf:type owl:Class ;
            rdfs:subClassOf cssv:Specification ;
            owl:disjointWith cssv:Standard ;
            rdfs:comment "A collection of interrelated and/or complementary specifications, standards or application profiles and the explanation of how they are combined, used or both."@en ;
            rdfs:isDefinedBy <https://data.europa.eu2sa/cssv> ;
            rdfs:label "Family"@en ;
            skos:definition "A collection of interrelated and/or complementary specifications, standards or application profiles and the explanation of how they are combined, used or both."@en ;
            skos:prefLabel "Family"@en .


###  https://data.europa.eu2sa/cssv#Specification
cssv:Specification rdf:type owl:Class ;
                   rdfs:subClassOf dcat:Dataset ;
                   rdfs:comment "Precise requirements that are needed for the implementation of a solution. A specification is not necessarily a standard."@en ;
                   rdfs:isDefinedBy <https://data.europa.eu2sa/cssv> ;
                   rdfs:label "Specification"@en ;
                   skos:definition "Precise requirements that are needed for the implementation of a solution. A specification is not necessarily a standard."@en ;
                   skos:prefLabel "Specification"@en .


###  https://data.europa.eu2sa/cssv#Standard
cssv:Standard rdf:type owl:Class ;
              rdfs:subClassOf dct:Standard ,
                              cssv:Specification ;
              rdfs:comment "Specification that has reached a certain maturity and widespread adoption and potentially endorsed."@en ;
              rdfs:isDefinedBy <https://data.europa.eu2sa/cssv> ;
              rdfs:label "Standard"@en ;
              skos:definition "Specification that has reached a certain maturity and widespread adoption and potentially endorsed."@en ;
              skos:prefLabel "Standard"@en .


###  https://schema.org/ContactPoint
sch:ContactPoint rdf:type owl:Class .


###  https://www.w3.org/TR/dx-prof/#Profile
prof:Profile rdf:type owl:Class ;
             rdfs:subClassOf dct:Standard .


#################################################################
#    Individuals
#################################################################

###  https://data.europa.eu2sa/cssv
<https://data.europa.eu2sa/cssv> rdf:type owl:NamedIndividual ;
                                 dct:description "This module provides the definitions for the Core Standards and Specifications Vocabulary."@en ;
                                 dct:title "Core Standards and Specifications Vocabulary"@en .


###  Generated by the OWL API (version 4.5.25.2023-02-15T19:15:49Z) https://github.com/owlcs/owlapi
